setup scaffolding

StackLean/Basic.lean
@@ -1,1 +1,76 @@
-def hello := "world"
+import Lean.Data.PersistentHashMap
+import Mathlib.Data.Multiset.Basic
+import Mathlib.Data.Multiset.AddSub
+import Mathlib.Data.Multiset.Dedup
+import Mathlib.Data.Finset.Basic
+import Aesop
+
+abbrev Word := Fin (2 ^ 256)
+
+inductive Slot where
+  | Var : Nat → Slot
+  | Lit : Word → Slot
+  | Junk : Slot
+  deriving BEq, Hashable, DecidableEq
+
+abbrev Stack := List Slot
+
+structure Target where
+  args : Stack
+  tail : Multiset Slot
+
+inductive Op where
+  | Swap     : Fin 16 → Op
+  | Dup      : Fin 16 → Op
+  | Pop      : Op
+  | Push     : Word → Op
+  | MarkJunk : Fin 1024 → Op
+
+inductive Err where
+  | StackTooDeep : Err
+  | StackTooShallow : Err
+
+def Stack.apply (stack : Stack) : Op → Except Err Stack
+  | .Swap idx =>
+      if h : idx < stack.length
+      then
+        let s := stack.set 0 stack[idx]
+        return s.set idx stack[0]
+      else throw .StackTooShallow
+  | .Dup idx =>
+      if h : idx < stack.length
+      then return (stack[idx] :: stack)
+      else throw .StackTooShallow
+  | .Pop =>
+      if stack.length > 0
+      then return stack.tail
+      else throw .StackTooShallow
+  | .Push v => return (.Lit v :: stack)
+  | .MarkJunk idx =>
+      if idx < stack.length
+      then return stack.set idx .Junk
+      else throw .StackTooShallow
+
+theorem apply_swap_inv (stack : Stack) (idx : Fin 16) (h : idx < stack.length) :
+  stack.apply (.Swap idx) >>= (·.apply (.Swap idx)) = .ok stack := by
+    simp_all [Stack.apply, pure, Except.pure]
+    sorry
+
+
+
+--def shuffle (stack : Stack) (target : Target) : Except Err Stack := do
+  --let (head, tail) := stack.splitAt target.args.length
+  ---- check if the current head matches the target head
+  --if head == target.args then
+    ---- check if any of the args are also required in the tail and not there yet
+    --let missing := (target.tail - (Multiset.ofList tail)).toFinset
+    --for slot in missing do
+      --match head.findIdx? (· == slot) with
+      --| .none => continue
+      --| .some idx =>
+        --if h : idx < 16 then
+          --return path ++ [Op.Dup ⟨idx, h⟩]
+        --else
+          --throw "Can't dup past 16..."
+    --return path
+  --return path
